Ordinary Differential Equations
===============================

Finite Difference Formulas
--------------------------

We define the backward difference operator $\nabla_h$ by:

.. math::

    \nabla_h f(a) = f(a) - f(a-h)

Repeated application gives:

.. math::

    \nabla_h^2 f(a) = \nabla_h (f(a) - f(a-h))
        = f(a) - f(a-h) -f(a-h) + f(a-2h)
        = f(a) - 2f(a-h) + f(a-2h)

    \nabla_h^3 f(a) = f(a) - 3f(a-h) + 3f(a-2h)-f(a-3h)

    \nabla_h^n f(a) = \sum_{k=0}^n \binom{n}{k}(-1)^k f(a-kh)

We can also derive a formula for $f(a+t)$ where $t$ is any real number,
independent of $h$:

.. math::

    f(a-h) = (1-\nabla_h) f(a)

    (1-\nabla_h)^{-1} f(a-h) = f(a)

    (1-\nabla_h)^{-1} f(a) = f(a+h)

    (1-\nabla_h)^{-n} f(a) = f(a+nh)

    (1-\nabla_h)^{-{t\over h}} f(a) = f(a+t)

Now we can express the following general integral using the function value from
either left ($f(a)$) or right ($f(a+h)$) hand side of the interval $h$:

.. math::

    \int_a^{a+h} f(t) \,\d t
        = \int_0^h f(a+t) \,\d t
        = \int_0^h (1-\nabla_h)^{-{t\over h}} f(a) \,\d t
        =

        = - {h\nabla_h\over (1-\nabla_h) \log(1-\nabla_h)}f(a) =

        = h \left(1+\half\nabla_h + {5\over 12}\nabla_h^2+{3\over8}
            \nabla_h^3+\cdots\right) f(a) =

        = - {h\nabla_h\over \log(1-\nabla_h)} (1-\nabla_h)^{-1}f(a)
        = - {h\nabla_h\over \log(1-\nabla_h)} f(a+h) =

        = h \left(1-\half\nabla_h - {1\over 12}\nabla_h^2-{1\over24}
            \nabla_h^3+\cdots\right) f(a+h)

Code::

    >>> from sympy import var, simplify, integrate
    >>> var("nabla t h")
    (nabla, t, h)
    >>> s = integrate((1-nabla)**(-t/h), (t, 0, h))
    >>> simplify(s)
    h*nabla/(-log(1 - nabla) + nabla*log(1 - nabla))
    >>> s.series(nabla, 0, 5)
    h + h*nabla/2 + 5*h*nabla**2/12 + 3*h*nabla**3/8 + 251*h*nabla**4/720 + O(nabla**5)
    >>> s2 = s*(1-nabla)
    >>> simplify(s2)
    -h*nabla/log(1 - nabla)
    >>> s2.series(nabla, 0, 5)
    h - h*nabla/2 - h*nabla**2/12 - h*nabla**3/24 - 19*h*nabla**4/720 + O(nabla**5)


Keeping terms only to third-order, we obtain:

.. math::

    \int_a^{a+h} f(t) \,\d t
        = - {h\nabla_h\over (1-\nabla_h) \log(1-\nabla_h)}f(a)
        \approx h \left(1+\half\nabla_h + {5\over 12}\nabla_h^2+{3\over8}
            \nabla_h^3\right) f(a)
        =

        = h f(a) + h\half\left(f(a)-f(a-h)\right)
            +h{5\over 12}\left(f(a)-2f(a-h)+f(a-2h)\right)+

            +h{3\over8}\left(f(a)-3f(a-h)+3f(a-2h)-f(a-3h)\right)
        =

        = h\left(1+\half+{5\over12}+{3\over8}\right)f(a)
          -h\left(\half+{2\cdot5\over12}+{3\cdot3\over8}\right)f(a-h) +

          +h\left({5\over12}+{3\cdot3\over8}\right)f(a-2h)
          -h\left({3\over8}\right)f(a-3h)
        =

        = h{55\over24}f(a) -h{59\over24}f(a-h) +
          h{37\over24}f(a-2h) -h{3\over8}f(a-3h)
        =

        = {h\over24}\left(55f(a) -59f(a-h) + 37f(a-2h) -9f(a-3h)\right)

Similarly:

.. math::

    \int_a^{a+h} f(t) \,\d t
        = - {h\nabla_h\over\log(1-\nabla_h)}f(a+h)
        \approx h \left(1-\half\nabla_h - {1\over 12}\nabla_h^2-{1\over24}
            \nabla_h^3\right) f(a+h)
        =

        = {h\over24}\left(9f(a+h) +19f(a) -5f(a-h) +f(a-2h)\right)

Code::

    >>> from sympy import var
    >>> var("f0 f1 f2 f3")
    (f0, f1, f2, f3)
    >>> nabla1 = f0 - f1
    >>> nabla2 = f0 - 2*f1 + f2
    >>> nabla3 = f0 - 3*f1 + 3*f2 - f3
    >>> 24*(f0 + nabla1/2 + 5*nabla2/12 + 3*nabla3/8)
    -59*f1 - 9*f3 + 37*f2 + 55*f0
    >>> 24*(f0 - nabla1/2 - nabla2/12 - nabla3/24)
    f3 - 5*f2 + 9*f0 + 19*f1

Integrating ODE
---------------

Set of linear ODEs can be written in the form:

.. math::
    :label: ode_eq

    {\d y\over\d r} = G y

For example for the Schr√∂dinger we have

.. math::

    y = \begin{pmatrix}
        P \\
        Q
        \end{pmatrix}

    G = \begin{pmatrix}
        0 & 1 \\
        -2(E-V) - {l(l+1)\over r^2} & 0 \\
        \end{pmatrix}

Now we need to choose a grid $r = r(t)$, where $t$ is some uniform grid. For
example $r = r_0 (e^t-1)$:

.. math::

    r_i = r_0 (e^{t_i} - 1)

    t_i = (i-1)h

where $i = 1, 2, 3, \dots, N$. We also need the derivative, for the exampe
above we get:

.. math::

    {\d r\over\d t} = r_0 e^t

Now we substitute this into :eq:`ode_eq`:

.. math::

    {\d y\over\d t} = {\d r\over\d t} G y

We can integrate this system from $a$ to $a+h$ on a uniform grid $t_i$:

.. math::

    y(a+h) = y(a) + \int_a^{a+h} {\d r\over\d t} G y\,\d t
        = y(a) + \int_a^{a+h} f(t)\,\d t

where $f(t) = {\d r\over\d t} G y$ and we use some method to approximate the
integral, see the previous section.

Radial Poisson Equation
-----------------------

Radial Poisson equation is:

.. math::
    :label: poisson-V

    V''(r) + {2\over r} V'(r) = -4\pi n(r)

The left hand side can be written as:

.. math::

    V'' + {2\over r} V'
        = {1\over r} \left(r V'' + 2V'\right)
        = {1\over r} \left(r V\right)''

So the Poisson equation can also be written as:

.. math::
    :label: poisson-rV

    (rV)'' = -4\pi r\, n

Now we determine the values of $V(0)$, $V'(0)$ and the behavior of
$V(\infty)$ and $V'(\infty)$. The equation determines $V$ up to an
arbitrary constant, so we set $V(\infty) = 0$ and now the potential $V$ is
determined uniquely.

The 3D integral of the (number) density is equal to the total (numeric) charge, which is equal to $Z$ (number of electrons). We can then use the Poisson equation to rewrite the integral in terms of $V$:

.. math::

    Z = \int n({\bf x}) \d^3 x
        = \int n(r) r^2\d\Omega\d r
        = \int_0^\infty 4\pi n(r) r^2\d r =

        = -\int_0^\infty (rV)'' r\d r =

        = \int_0^\infty (rV)'\d r - [(rV)'r]_0^\infty =

        = [rV]_0^\infty - [(rV)'r]_0^\infty =

        = [rV - (rV)'r]_0^\infty =

        = -[V'r^2]_0^\infty =

        = \lim_{r\to0} V'(r)r^2 -\lim_{r\to\infty} V'(r)r^2

Let

.. math::

    \lim_{r\to0} V'(r)r^2 = C

Then around $r\to0$ we get $V'(r) = {C\over r^2}$ and $V(r) = -{C\over r}+D$
(for some constant $D$). As such, $C$ is a point charge (delta function) at
the origin. From now on, we will assume no point charge, i.e. $C=0$.

In the limit $r\to\infty$, we get the equation:

.. math::

    V'(r) = -{Z-C\over r^2} = -{Z\over r^2}

by integrating (and requiring that $V$ vanished in infinity to get rid of the
integration constant), we get for $r\to\infty$:

.. math::

    V(r) = {Z\over r}

Integrating :eq:`poisson-rV` directly, we get:

.. math::

    [(rV)']_0^\infty = -4\pi\int_0^\infty r n(r) \d r

    [V + rV']_0^\infty = -4\pi\int_0^\infty r n(r) \d r

We already know that $V'$ behaves like $-{Z\over r^2}$ in infinity,
so $rV'$ vanishes. Requiring $V$ itself to
vanish in infinity, the left hand side simplifies to $-V(0)$ and we get:

.. math::

    V(0) = 4\pi\int_0^\infty r n(r) \d r

Last thing to determine is $V'(0)$. To do that, we expand the charge density
and potential (and it's derivatives) into a series around the origin:

.. math::

    n(r) = n_0 + n_1 r + n_2 r^2 + \cdots = \sum_{k=0}^\infty n_k r^k

    V(r) = V_0 + V_1 r + V_2 r^2 + \cdots = \sum_{k=0}^\infty V_k r^k

    V'(r) = \sum_{k=1}^\infty V_k k r^{k-1}

    V''(r) = \sum_{k=2}^\infty V_k k(k-1) r^{k-2}

And substitute into the equation :eq:`poisson-V`:

.. math::

    \sum_{k=2}^\infty V_k k(k-1) r^{k-2} +
        {2\over r}\sum_{k=1}^\infty V_k k r^{k-1} =
        -4\pi \sum_{k=0}^\infty n_k r^k

    \sum_{k=2}^\infty V_k k(k-1) r^{k-2} + {2\over r} V_1 +
        {2\over r}\sum_{k=2}^\infty V_k k r^{k-1} =
        -4\pi \sum_{k=0}^\infty n_k r^k

    \sum_{k=2}^\infty V_k k(k-1) r^{k-2} + {2\over r} V_1 +
        \sum_{k=2}^\infty 2V_k k r^{k-2} =
        -4\pi \sum_{k=0}^\infty n_k r^k

    {2\over r} V_1 +
        \sum_{k=2}^\infty V_k k\left((k-1) +2\right)r^{k-2}
        =
        -4\pi \sum_{k=0}^\infty n_k r^k

    {2\over r} V_1 +
        \sum_{k=2}^\infty V_k k(k+1)r^{k-2}
        =
        -4\pi \sum_{k=0}^\infty n_k r^k

    {2\over r} V_1 +
        \sum_{l=0}^\infty V_{l+2} (l+2)(l+3)r^l
        =
        -4\pi \sum_{k=0}^\infty n_k r^k

    {2\over r} V_1
        =
        -\sum_{k=0}^\infty \left(4\pi n_k+V_{k+2} (k+2)(k+3)\right) r^k

We now multiply the whole equation by $r$ and then set $r=0$. We get
$V_1 = 0$, so $V'(0) = V_1 = 0$. We put it back into the equation to get:

.. math::

    \sum_{k=0}^\infty \left(4\pi n_k+V_{k+2} (k+2)(k+3)\right) r^k = 0

This must hold for all $r$, so we get the following set of equations for $k=0,
1, \cdots$:

.. math::

    4\pi n_k+V_{k+2} (k+2)(k+3) = 0

from which we express $V_k$ for all $k \ge 2$.
We already know the values for $k=1$ and
$k=0$ from earlier, so overall we get:

.. math::

    V_0 = 4\pi\int_0^\infty r n(r) \d r

    V_1 = 0

    V_{k+2} = -{4\pi n_k\over (k+2)(k+3)}

in particular:

.. math::

    V_2 = - {4\pi n_0\over 6} = -{2\pi\over 3} n_0

    V_3 = - {4\pi n_1\over 12} = -{\pi\over 3} n_1

    V_4 = - {4\pi n_2\over 20} = -{\pi\over 5} n_2

    V_5 = - {4\pi n_3\over 30} = -{2\pi\over 15} n_3

    \cdots

So we get the following series expansion for $V$ and $V'$:

.. math::

    V = V_0 -{2\pi\over 3} n_0 r^2 -{\pi\over 3} n_1 r^3-{\pi\over 5} n_2 r^4
        -{2\pi\over 15} n_3 r^5 - \cdots

    V' = -{4\pi\over 3} n_0 r -\pi n_1 r^2-{4\pi\over 5} n_2 r^3
        -{2\pi\over 3} n_3 r^4 - \cdots

Examples
~~~~~~~~

It is useful to have analytic solutions to test the numerical solvers. Here we
present a few.

Gaussian Charge
^^^^^^^^^^^^^^^

The Gaussian charge is simply a Gaussian, normalized in such a way that the
total charge is $Z$:

.. math::
    :label: gauss_charge

    n(r) = {Z\alpha^3 \over \pi^{3\over2} } e^{-\alpha^2 r^2}

Let us verify the normalization by calculating the total charge $Q$:

.. math::

    Q = \int n({\bf x}) \d^3 x
        = 4\pi \int_0^\infty n(r) r^2 \d r =

    = 4\pi \int_0^\infty {Z\alpha^3 \over \pi^{3\over2} } e^{-\alpha^2 r^2}
        r^2 \d r =

    = {4 Z \alpha^3 \over \sqrt\pi} \int_0^\infty e^{-\alpha^2 r^2} r^2 \d r =

    = {4 Z \alpha^3 \over \sqrt\pi} {\sqrt\pi\over 4\alpha^3} = Z

So the total charge is $Q=Z$, as expected. Code::

    >>> from sympy import var, integrate, exp, Symbol, oo
    >>> var("r")
    r
    >>> alpha=Symbol("alpha", positive=True)
    >>> integrate(exp(-alpha**2*r**2)*r**2, (r, 0, oo))
    sqrt(pi)/(4*alpha**3)


Now we calculate the potential $V(r)$ from the Poisson equation
:eq:`poisson-rV`:

.. math::

    \left(rV(r)\right)'' = -4\pi r n(r)
        = -{4\alpha^3 r Z\over \sqrt\pi } e^{-\alpha^2 r^2}

    \left(rV(r)\right)' = {2 Z\alpha\over \sqrt\pi } e^{-\alpha^2 r^2} + A

    r V(r) = Z \,\mbox{erf}(\alpha r) + Ar + B

    V(r) = Z \,{\mbox{erf}(\alpha r) \over r} + A + {B\over r}

We have two integration constants $A$ and $B$. We fix the potential using the
condition $V(\infty) = 0$, which implies $A=0$. The other constant $B$ is a
point charge at the origin, which in our case :eq:`gauss_charge` is zero, so
$B=0$.

We finally obtain the potential:

.. math::

    V(r) = Z \,{\mbox{erf}(\alpha r) \over r}

We can calculate the electrostatic self-energy, i.e. the energy of
interaction of the charge $n(r)$ with the potential generated by this
charge $V(r)$:

.. math::

    E_\mathrm{self} =
    \half \int n({\bf x}) V({\bf x}) \d^3 x
        = {4\pi\over2} \int_0^\infty n(r) V(r) r^2 \d r =

    = 2\pi \int_0^\infty {Z\alpha^3 \over \pi^{3\over2} } e^{-\alpha^2 r^2}
        Z \,{\mbox{erf}(\alpha r) \over r} r^2 \d r =

    = {2 Z^2 \alpha^3 \over \sqrt\pi}
        \int_0^\infty e^{-\alpha^2 r^2} \mbox{erf}(\alpha r) r \d r =

    = {2 Z^2 \alpha^3 \over \sqrt\pi} {\sqrt 2 \over 4\alpha^2} =

    = {Z^2 \alpha\over \sqrt{2\pi}}

Code::

    >>> from sympy import var, integrate, exp, Symbol, oo, erf
    >>> var("r")
    r
    >>> alpha=Symbol("alpha", positive=True)
    >>> integrate(exp(-alpha**2*r**2)*erf(alpha*r)*r, (r, 0, oo))
    sqrt(2)/(4*alpha**2)


Exponential Charge
^^^^^^^^^^^^^^^^^^

The exponential charge is simply an exponential, normalized in such a way that
the total charge is $Z$:

.. math::
    :label: exp_charge

    n(r) = {Z\alpha^3 \over 8\pi} e^{-\alpha r}

Let us verify the normalization by calculating the total charge $Q$:

.. math::

    Q = \int n({\bf x}) \d^3 x
        = 4\pi \int_0^\infty n(r) r^2 \d r =

    = 4\pi \int_0^\infty {Z\alpha^3 \over 8\pi} e^{-\alpha r}
        r^2 \d r =

    = {Z \alpha^3 \over 2} \int_0^\infty e^{-\alpha r} r^2 \d r =

    = {Z \alpha^3 \over 2} {2\over\alpha^3} = Z

So the total charge is $Q=Z$, as expected.

Now we calculate the potential $V(r)$ from the Poisson equation
:eq:`poisson-rV`:

.. math::

    \left(rV(r)\right)'' = -4\pi r n(r)
        = -{Z\alpha^3 \over 2} r e^{-\alpha r}

    V(r) = - Z \left({\alpha\over2} + {1\over r}\right) e^{-\alpha r} + A + {B\over r}


Similarly as for the Gaussian charge, we require the potential $V(r)$ to vanish
at infinity, which implies $A=0$. Then we calculate the point charge at the
origin:

.. math::

    C = \lim_{r\to0} V'(r)r^2 =

    = \lim_{r\to0}
    \half \left(- 2 B e^{\alpha r} + Z \alpha r \left(\alpha r + 1\right)
    + Z \left(\alpha r + 2\right)\right) e^{- \alpha r} =

    = Z - B

We do not have any point charge at the origin, so $C=Z - B = 0$, from which it
follows $B = Z$. We finally obtain:

.. math::

    V(r) = - Z \left({\alpha\over2} + {1\over r}\right) e^{-\alpha r}
        + {Z \over r}
        = Z \left({1-e^{-\alpha r} \over r} - {\alpha e^{-\alpha r}
            \over 2}\right)

Let us calculate the self-energy:

.. math::

    E_\mathrm{self} =
    \half \int n({\bf x}) V({\bf x}) \d^3 x
        = {4\pi\over2} \int_0^\infty n(r) V(r) r^2 \d r =

    = 2\pi \int_0^\infty
    {Z\alpha^3 \over 8\pi} e^{-\alpha r}
    Z \left({1-e^{-\alpha r} \over r} - {\alpha e^{-\alpha r}
            \over 2}\right)
    r^2 \d r =

    = {Z^2 \alpha^3 \over 4}
        \int_0^\infty e^{-\alpha r}
       \left({1-e^{-\alpha r} \over r} - {\alpha e^{-\alpha r}
            \over 2}\right)
        r^2 \d r =

    = {Z^2 \alpha^3 \over 4}
        \left({5\over 8\alpha^2}\right) =

    = {5Z^2 \alpha \over 32}

Code::

    >>> from sympy import var, integrate, exp, Symbol, oo
    >>> var("r Z B")
    (r, Z, B)
    >>> alpha=Symbol("alpha", positive=True)
    >>> integrate(exp(-alpha*r)*r**2, (r, 0, oo))
    2/alpha**3
    >>> V = integrate(-Z*alpha**3/2 * r * exp(-alpha*r), r, r)/r
    >>> V.simplify()
    -Z*(alpha*r + 2)*exp(-alpha*r)/(2*r)
    >>> ((V+B/r).diff(r)*r**2).simplify()
    (-2*B*exp(alpha*r) + Z*alpha*r*(alpha*r + 1) + Z*(alpha*r +
    2))*exp(-alpha*r)/2
    >>> ((V+B/r).diff(r)*r**2).limit(r, 0)
    -B + Z
    >>> integrate(exp(-alpha*r)*((1-exp(-alpha*r))/r-alpha*exp(-alpha*r)/2)*r**2, (r, 0, oo))
    5/(8*alpha**2)

Piecewise Polynomial Charge
^^^^^^^^^^^^^^^^^^^^^^^^^^^

We will use a second-derivative continuous piecewise polynomial for $n(r)$,
normalized in such a way that the total charge is $Z$:

.. math::
    :label: poly_charge

    n(r) = \begin{cases}
    -21Z(r-r_c)^3(6r^2+3rr_c+r_c^2)/(5\pi r_c^8) &\quad\mbox{for $0\le r \le r_c$}\cr
    0&\quad\mbox{for $r>r_c$}\cr
    \end{cases}

Let us verify the normalization by calculating the total charge $Q$:

.. math::

    Q = \int n({\bf x}) \d^3 x
        = 4\pi \int_0^\infty n(r) r^2 \d r =

    = 4\pi \int_0^{r_c} -21Z(r-r_c)^3(6r^2+3rr_c+r_c^2)/(5\pi r_c^8)
        r^2 \d r =

    = Z

So the total charge is $Q=Z$, as expected.

Now we calculate the potential $V(r)$ from the Poisson equation
:eq:`poisson-rV`:

.. math::

    \left(rV(r)\right)'' = -4\pi r n(r)
        = 4\pi r \cdot 21Z(r-r_c)^3(6r^2+3rr_c+r_c^2)/(5\pi r_c^8)

    V(r) = \begin{cases}
    \frac{Z r^{2}}{5 r_{c}^{8}} \left(9 r^{5} - 30 r^{4} r_{c} + 28
    r^{3} r_{c}^{2} - 14 r_{c}^{5}\right) + A_1 + {B_1\over r}
    &\quad\mbox{for $0\le r \le r_c$}\cr
    A_2 + {B_2\over r}&\quad\mbox{for $r>r_c$}\cr
    \end{cases}


Similarly as for the Gaussian charge, we require the potential $V(r)$ to vanish
at infinity, which implies $A_2=0$. Then we calculate the point charge at the
origin:

.. math::

    C = \lim_{r\to0} V'(r)r^2 =

    = \lim_{r\to0}\left(
    - B_1 + \frac{63 Z r^{8}}{5 r_{c}^{8}} - \frac{36 Z}{r_{c}^{7}} r^{7} +
      \frac{28 Z}{r_{c}^{6}} r^{6} - \frac{28 Z r^{3}}{5 r_{c}^{3}}
      \right)

    = -B_1

We do not have any point charge at the origin, so $C=-B_1 = 0$, from which it
follows $B_1 = 0$. Then $B_2$ is calculated from the condition of a continuous
first derivative at $r=r_c$:

.. math::

    V'(r_c) = \begin{cases}
    -{Z\over r_c^2} &\quad\mbox{for $0\le r \le r_c$}\cr
    -{B_2\over r_c^2}&\quad\mbox{for $r>r_c$}\cr
    \end{cases}

So $B_2=Z$. Finally, $A_1$ is calculated from the continuous
values of $V(r_c)$:

.. math::

    V(r_c) = \begin{cases}
    A_1-{7Z\over 5r_c} &\quad\mbox{for $0\le r \le r_c$}\cr
    {Z\over r_c}&\quad\mbox{for $r>r_c$}\cr
    \end{cases}

which implies $A_1={12Z\over 5r_c}$. We finally obtain:

.. math::

    V(r) = \begin{cases}
    \frac{Z}{5 r_{c}^{8}} \left(9r^7 - 30r^6r_c + 28r^5r_c^2 - 14r^2r_c^5
        + 12 r_c^7\right) &\quad\mbox{for $0\le r \le r_c$}\cr
    {Z\over r}&\quad\mbox{for $r>r_c$}\cr
    \end{cases}

Let us calculate the self-energy:

.. math::

    E_\mathrm{self} =
    \half \int n({\bf x}) V({\bf x}) \d^3 x
        = {4\pi\over2} \int_0^\infty n(r) V(r) r^2 \d r =

    = 2\pi \int_0^{r_c}
    -21Z(r-r_c)^3(6r^2+3rr_c+r_c^2)/(5\pi r_c^8)
    \frac{Z}{5 r_{c}^{8}} \left(9r^7 - 30r^6r_c + 28r^5r_c^2 - 14r^2r_c^5
        + 12 r_c^7\right)
    r^2 \d r =

    = {15962 Z^2 \over 17875 r_c}

Let us also calculate the following integral:

.. math::

    I_g =
    \int n({\bf x}) \left({Z\over r}-V({\bf x})\right) \d^3 x
        = 4\pi \int_0^\infty n(r) \left({Z\over r}-V(r)\right) r^2 \d r =

    = {10976 Z^2 \over 17875 r_c}

Which agrees with [Pask2012]_, equation (10c). The following integral over the
sphere of radius $r_c$:

.. math::

    I_{sph} =
    \int_{\Omega: r < r_c} \left({Z\over r}-V({\bf x})\right) \d^3 x
        = 4\pi \int_0^{r_c} \left({Z\over r}-V(r)\right) r^2 \d r =

    = {14 \pi Z r_c^2 \over 75}

Again in agreement with [Pask2012]_, the paragraph after equation (17).


Code::

    >>> from sympy import var, pi, integrate, solve
    >>> var("r r_c Z A B")
    (r, r_c, Z, A, B)
    >>> n = -21*Z*(r-r_c)**3*(6*r**2+3*r*r_c+r_c**2)/(5*pi* r_c**8)
    >>> 4*pi*integrate(n*r**2, (r, 0, r_c))
    Z
    >>> V = integrate(-4*pi*r*n, r, r)/r
    >>> V.simplify()
    Z*r**2*(9*r**5 - 30*r**4*r_c + 28*r**3*r_c**2 - 14*r_c**5)/(5*r_c**8)
    >>> ((V+A+B/r).diff(r)*r**2).simplify()
    -B + 63*Z*r**8/(5*r_c**8) - 36*Z*r**7/r_c**7 + 28*Z*r**6/r_c**6 - 28*Z*r**3/(5*r_c**3)
    >>> (V+A).diff(r).subs(r, r_c)
    -Z/r_c**2
    >>> (V+A).subs(r, r_c)
    A - 7*Z/(5*r_c)
    >>> A = solve((V+A).subs(r, r_c)-Z/r_c, A)[0]
    >>> A
    12*Z/(5*r_c)
    >>> V = V + A
    >>> V.simplify()
    Z*(r**2*(9*r**5 - 30*r**4*r_c + 28*r**3*r_c**2 - 14*r_c**5) + 12*r_c**7)/(5*r_c**8)
    >>> 2*pi*integrate(n*V*r**2, (r, 0, r_c))
    15962*Z**2/(17875*r_c)
    >>> 4*pi*integrate(n*(Z/r-V)*r**2, (r, 0, r_c))
    10976*Z**2/(17875*r_c)
    >>> 4*pi*integrate((Z/r-V)*r**2, (r, 0, r_c))
    14*pi*Z*r_c**2/75

Alternatively, one can also calculate this using a ``Piecewise`` function::


    >>> from sympy import var, pi, integrate, solve, Piecewise, oo, Symbol
    >>> var("r Z A B")
    (r, Z, A, B)
    >>> r_c = Symbol("r_c", positive=True)
    >>> n = Piecewise((-21*Z*(r - r_c)**3*(6*r**2 + 3*r*r_c + r_c**2)/(5*pi*r_c**8), r <= r_c), (0, True))
    >>> 4*pi*integrate(n*r**2, (r, 0, oo))
    Z
    >>> V = integrate(-4*pi*r*n, r, r)/r
    >>> V.simplify()
    Piecewise((Z*r**2*(9*r**5 - 30*r**4*r_c + 28*r**3*r_c**2 - 14*r_c**5)/(5*r_c**8), r <= r_c), (0, True))
    >>> ((V+A+B/r).diff(r)*r**2).simplify()
    Piecewise((-B + 63*Z*r**8/(5*r_c**8) - 36*Z*r**7/r_c**7 + 28*Z*r**6/r_c**6 - 28*Z*r**3/(5*r_c**3), r <= r_c), (-B, True))
    >>> (V+A).diff(r).subs(r, r_c)
    -Z/r_c**2
    >>> (V+A).subs(r, r_c)
    A - 7*Z/(5*r_c)
    >>> A = solve((V+A).subs(r, r_c)-Z/r_c, A)[0]
    >>> A
    12*Z/(5*r_c)
    >>> V = V + Piecewise((A, r <= r_c), (0, True))
    >>> V.simplify()
    Piecewise((Z*(r**2*(9*r**5 - 30*r**4*r_c + 28*r**3*r_c**2 - 14*r_c**5)/r_c**7 + 12)/(5*r_c), r <= r_c), (0, True))
    >>> 2*pi*integrate(n*V*r**2, (r, 0, oo))
    15962*Z**2/(17875*r_c)
    >>> 4*pi*integrate(n*(Z/r-V)*r**2, (r, 0, oo))
    10976*Z**2/(17875*r_c)

.. [Pask2012] Pask, J. E., Sukumar, N., Mousavi, S. E. (2012). Linear scaling solution of the all-electron Coulomb problem in solids. International Journal for Multiscale Computational Engineering, 10(1), 83‚Äì99.  doi:10.1615/IntJMultCompEng.2011002201
